\subsection{Trigonometric formulae and polar form}

Page 672

De Moive's theorem
$z^n=r^n cis(n\cdot\theta)$
with binomial theorem
$(a+b)^n=nCr(n,0)a^n+(n,1)a^{n-1}b^1+...$
$+(n,k)a^kb^{n-k}+....+(n,n)b^n$
and trigonometric formulas, 
trigonometric integral
geometric progression
$a_1+a_q+...+aq^{n-1}=q_1(1-q^n)$

Example let $z=1\cdot cis(\theta)$
a) $z^n=(1 cis\theta)^n=1^n cis(n\theta)=cis(n\theta)$
$\frac{1}{z}^n=z^{-n}=1^{-n}cos(-n\theta)=cis(-n\theta)$
$=cos(-n\theta)+i sin(-n\theta)$
$cos(+n\theta)-isin(n\theta)$
Now $z^n-\frac{1}{z}^n=(cos(n\theta)+isin \theta n)-(cos\ntheta-i sinn\theta)$
$=z i sin(n\theta)$
b) Simplify $(z-\frac{1}{z})^5$
$z^5+5z^4(z^-1)^1+10\cdot z^3(z^{-1})^2+10\cdot z^2(z^{-1})^3+5z(z^{-1})^4+(z^{-1})^5$
$=z^5-5^3+10z^1-10z^{-1}+5z^{-3}-z^{-5}$
$=1\cdot(z^5-\frac{1}{z}5)-5(z^3-\frac{1}{z^3}+10(z-\frac{1}{z})$
$=zisin(5\cdot \theta)\cdot 5(2isin(3\cdot0)+10(2isin1\theta)$
c) $\int sin^5\theta d\theta=?$

$(z-\frac{1}{z})^5=(2i sin\theta)^5$
$2isin5\theta-10isin3\theta+20isin\theta=2^5i^5sin5\theta$
$sin5\theta-5sin3\theta+10sin\theta-16sin5\theta$
$i^4=1$

Now
$\int sin^5\theta d\theta$
$\int \frac{1}{16}sin(5\theta)-5sin(3\theta)+10sin(\theta) d\theta$
$\frac{1}{16}(-cos(5\theta)\cdot\frac{1}{5}-5(-cos(3\theta)\frac{1}{3}+10(-cos\theta))+C$
$=-\frac{cos5\theta}{80}+\frac{5cos3\theta}{48}-\frac{5}{8}cos\theta +C$

p 674 ex 2-4
ex 2 $z=w5\theta+isin-\theta$
a) $z^4=(cos\theta+i sin\theta)^4$
$1\cdot cos^4\theta+4\cdot cos^3\theta i sin\theta+b cos^2(i sin\theta)^2+4cos^1\theta(i sin\theta)^3+(i sin\theta)^4$
$=cos^44icos^3\theta sin\theta-6 cos^2 sin^2\theta-4icos\theta sin^-3\theta+i sin^4\theta$
Real part = $cos^4\theta-6cos^2\theta sin^2\theta$
Imaginary part $=4i cos^3sin-4icos\theta sin^-3\theta+isin^4\theta$
2b) $z=cos(x)+isin(x)$
$z^4=1^4(cis(4x))=cos(4x)+isin(4x)$
so real part of $z^4=cos(4x)$
and imaginary $z^4=sin(4x)$
a) gives 
real part $cos(4x)=cos^4x-6cos^2x\cdot sin^2x+sin^4x$
ii) Imaginary part
$sin(4x)=4cos^3x\cdot sin(x)-4cos(x)\cdot sin^3x$
c) $tan(4x)=\frac{sin(4x)}{cos(4x)}substitute$
$=\frac{4cos^3x\cdot sin(x)-4cos(x)\cdot sin^3x}{cos^4x-6cos^2x\cdot sin^2x+sin^4x$
cancel by $cos^4x$
$=\frac{4\cdot\frac{sin(x)}{cos(x)}-4\cdot\frac{sin^3x}{cos^3x}}{1-6\cdot\frac{sin^2x}{cps^2x}+\frac{sin^4x}{cos^4x}}=\frac{4\cdot tan x-4 tan^4x}{1-6tan^2x+tan^4x}$
$=RHS$
ex 3. let $z=e^{i\theta}=1\cdot cis(\theta)$
