\subsection{Fundamental theorem of algebra}
HL p 184

A polynomial $f(x)=a_nx^n+a_{n-1}x^{n-1}+...+a_2x^2+a_1x+a_0,a_n\neq 0$

Has atleast one zeroe $\omega$ from complex number set so that $f(\omega)=0$.
Factored form $f(x)=a_n\cdot (x-\omega_1)\cdot (x-\omega_2)\cdot ...(x-\omega_n)$
where $\omega_1,\omega_2,...$ are zeroes.
Conjugate root (=solution, zeroe) theorem.
If $f(x)$ has zero z then it has also root conjugate $z^*$.

Sum and product of roots:
$x_1+x_2+x_3=\frac{-b}{a} or (\frac{-a_{n-1}}{a_n})$ where $ax^3+bx^2+cx+d=0$
$x_1\cdot x_2\cdot x_3=\frac{-d}{a} or ((-1)^n\cdot \frac{a_0}{a_n})$
$x_1x_2+x_1+x_3+x_2x_3=\frac{c}{a} or \frac{a_{n-2}}{a_n}$

Example find the root of.
$x^4-2x^3+6x^2-2x+5=0$
Let's try $x=1$, substitution gives
$i^4-2\cdot(i^3)+6i^2-2(i)+5=0$
$+1-2(i\cdot (-1))-6-2i+5=0$
$1+2i-6-2i+5=0$
$0=0$ so i is one of the 4 solutions.
Conjugate root theorem tells us that conjugate of $i=-i$ is also a root.
$f(x)$ is divisible by $1\cdot(x-1)\cdot(x-(-1))$
$=x^2+xi-ix-i^2=x^2-i^2=x^2-(-1)=x^2+1$
Let's do long division $\frac{x^4-2x^3+6x^2-2x+5}{x^2+1}$
$remainder=0$ divisible!
quotient $x^2-2x+5$ and it has zeroes solved by quadr.
$x=\frac{-(-2)\pm\sqrt{(-2)^2-4\cdot 1\cdot 5}}{2}=\frac{4\pm\sqrt{4-20}}{2}$
$=\frac{4\pm\sqrt(-16)}{2}$
$=\frac{4\pm\sqrt{16\cdot i^2}}{2}=\frac{4\pm4i}{2}=2\pm2i$
Ans: $x=1,x=-1,x=2+2i,x=2-2i$
Example 2. Find the sum of roots of
$4x^3-2x^2+7x+9=0$
formula $x_1+x_2+x_3=\frac{-b}{a}=\frac{-(-2)}{4}=\frac{1}{2}$
b) Given that $x+2$ is a factor of $x^3-6x^2+25x+82$. Find all the zeroes/roots.
Synthetic division since $x+2$ is a factor for $x+2=0,x=-2$
$\frac{1\cdot x^3-6x^2+25x+82}{x+2}=1x^2-8x+41$
So it has zeroes $x=\frac{8\pm\sqrt{8^2-5\cdot 1\cdot 41}}{2}$
$=\frac{8\pm\sqrt{100}}{2}=\frac{8\pm\sqrt{100\cdot i^2}}{2}=\frac{8\pm10i}{2}=4\pm5i$
Ans: $x=-2,x=4+5i,x=4-5i$
p 194 ex 1a, 2a and p 190 1a,1b,3a,5a.
1. a. $f(x)=x^4-3x^3+2x^2-5x+4$
cum of roots=$\frac{-a_{n-1}}{a_n}=\frac{-(-3)}{1}=3$
product of roots=$(-1)^n(\frac{a_0}{a_n})=(-1)^4\frac{4}{1}=4$
2a) $4x^3-2x^2+1\cdot x-7=10$
$4x^3-2x^2+1\cdot x-17=0$
sum of roots $=\frac{-a_{n-1}}{a_n}=\frac{-(-2)}{4}=\frac{1}{2}$
product of roots $=(-1)^n(\frac{a_0}{a_n})=(-1)^3(\frac{-17}{4})=\frac{-17}{4}$
2c) $10\cdot x_1 +10\cdot x_2+ 10\cdot x_3=10\cdot (sum)=10\cdot(1/2)=5$

