\documentclass{article}
\usepackage{graphicx} % Required for inserting images
\usepackage{hyperref}
\usepackage{graphicx} % Required for inserting images
\usepackage{mathtools,amssymb,amsthm}

\title{The day's notes}
\author{Samuel Hautam√§ki}
%\date{October 2025}
\begin{document}
\subsection{The integrating factor}
HL p 544
\obeylines
Is a method of solvind differential equation is case 
$\frac{dy}{dx}+P(x)\cdot y=Q(x)$
where $y=y(x)$ is a function of x
multiply by $I(X)=e^{\int P(x)dx}$
since $I'(x)=I(x)\cdot P(x)$
gives
$f(x)\cdot \frac{dy}{dx}+I(x) P(x)\cdot y=I(x) \cdot Q(x)$ 
$\int (I(x)\cdot\frac{dy}{dx}+I'(x)\cdot y)d=\int (I(x)\cdot Q(x)) d$
product rule of differentiation.
$\int D(I\cdot y) d= \int (I(x)\cdot Q(x)) d$
so $I\cdot y=\int (I(x) \cdot Q(x)) dx$
Example find the general solution to
$\frac{dy}{dx}-\frac{2}{x}\cdot y=x^3$
so $P(x)=-\frac{2}{x} Q=(x)=x^3$
integrating factor $I(x)=e^{\int(-2/x dx)}=e^{-2\cdot ln(x)}=e^{ln(x^{-2}}=x^{-2}$
$\frac{dy}{dx}-\frac{2}{x}\cdot y=x^3$
$\frac{d}{dx}(y\cdot x^{-2})-\frac{2}{x}\cdot y\cdot x^{-2}=x^3\cdot x^{-2}$
$(d(y\cdot x^{-2}-\frac{2}{x}\cdot y\cdot x^{-2}dx=x^3\cdot x^{-2}dx)$
$\int(dy x^{-2}-\frac{2}{x}\cdot y\cdot x^{-2})dx=\int x dx$
product ruel fo diff
$I(x)\cdot P(x)=\frac{1}{2}x^2+c$
$y\cdot x^{-2}=\frac{1}{2}x^2+c$
$y=\frac{1}{2}x^4+c\cdot x^2$
Ans: $y=\frac{1}{2}x^4+c\cdot x^2$ where c is constant of integration

ex 1., p 545
1a) $y'+y=e^x$
$\frac{dy}{dx}+1\cdot y=e^x$ integationg factor method
$p(x)=1$ and $Q(x)=e^x$ so $I(x)=e^{\int 1dx}=e^x$
$\frac{dy}{dx}+1\cdot y=e^x$
$\frac{dy}{dx}\cdot e^x+e^x1\cdot y=e^x\cdot e^x$
$\int(dy\cdot e^x+e^x\cdot y)dx=\int e^{2x} dx$
$\int D(y\cdot e^x)dx = e^{2x}\cdot(\frac{1}{2})+C$
$y\cdot e^x=e^{2x}\cdot (\frac{1}{2})+C$
$y=\frac{e^{2x}\cdot(\frac{1}{2})+C}{e^x}$
$y=\frac{1}{2}e^x+c\cdot e^{-x}$
1b) $(x-1)\cdot y'=y-x^2\cdot y$
$(x-1)\cdot y'=y\cdot(1-x^2)$
$y'=y\cdot \frac{1-x^2}{x-1}$
$y'=y\cdot \frac{(1-x)(1+x)}{-(-x+1)}$(cancel)
$y'=y\cdot (-(1+x)$
$y'+(1+x)\cdot y=0$
$P(x)=1+x$ and $Q(x)=0$
integrating factor $I(x)e^{\int(1+x)dx}=e^{x+1/2\cdot x^2}$
...
$I(x)\cdot y=\int (0\cdot e^{x+ 1/2\cdot x^2}dx$
$I(x\cdot y=\int 0dx$
$I(x)\cdot y=c$
$Ans: y=\frac{c}{e^{x+1/2\cdot x^2}}$
1c) $x\cdot y'+y=x^2+1$
$y'+\frac{1}{x}\cdot y=x\frac{1}{x}$
$p(x)=\frac{1}{x}$ so integrating factor $I(x)=e^{\int 1/x dx}=e^{ln(x)=x}$
im already lost.



\end{document}
