\documentclass{article}
\usepackage{graphicx} % Required for inserting images
\usepackage{hyperref}
\usepackage{mathtools,amssymb,amsthm}

\title{The day's notes}
\author{Samuel Hautam√§ki}
%\date{October 2025}
\begin{document}
\subsection{Revision of integration = antidifferentiation}
\obeylines
$F(x)=\int f(x) dx$ as $F'(x)=f(x)$
rules:
$\int c dx=c\int 1 dx=c\cdot x+C$
where c and C are constants.
$\int x^n dx=n\cdot x^{n-1}=\frac{1}{n+1}\cdot x^{n+1}+C,n\neq-1$
$\int x^{-1}dx=\int\frac{1}{x}dx=ln|x|+C$
$\int ((f(x))^n\cdot f'(x))dx=\frac{1}{n+1}\cdot (f(x))^{n+1}+c$
as you integrate, inner funcion must have a derivative and it drops out
note that multiplication or division is inner function's drivative or should be simplified first.
undefinite integral looks like $\int x dx=\frac{1}{2}x^2+c$
and defined integral looks like
$\int_{a}^{b}f(x) dx=F(b)-F(a)$
use minus with brackets, no need for C
Example
$\int_{0}^{1}(5x^3-4x^2-x+8)dx=$
$[5\cdot \frac{1}{4}\cdot x^4-4\cdot\frac{1}{3}x^3-\frac{1}{2}x^2+8x]+C$
$=(\frac{5}{4}1^4-\frac{4}{3}1^3-\frac{1}{2}1^2+8\cdot1)-(\frac{5}{4}\cdot 0-0-0+0)=\frac{89}{12}$
Example 2.
$\int_{2}^{3}(2\cdot x-5)^6dx$
paper2:$\frac{1}{7}$
paper 1: $\int_{2}^{3}(2\cdot x-5)^6dx=\frac{1}{2}\cdot\int_{2}^{3}(2\cdot(2x-5)^6)dx$
$=\frac{1}{2}[\frac{1}{7}(2x-5)^7]$ since 2 is inner function's derivaive
$=\frac{1}{2\cdot7}((2\cdot 3-5)^7-(2\cdot 2-5)^7)$
$=\frac{1}{14}(1-(-1))=\frac{2}{14}=\frac{1}{7}$
1. $\int2x^3dx$
$2\cdot\frac{1}{4}x^4=\frac{1}{2}x^4+C$
2. $\int \frac{3}{x^3}dx=3\int x^{-3}dx=3\cdot(\frac{1}{2}x^{-3+1})+c$
$=\frac{-3}{2}x^{-2}+c=\frac{-3}{2x^2}+c$
3. $\int \frac{1}{4x}dx=\int(\frac{1}{4}\cdot x^{-4})dx=\frac{1}{4}\cdot\frac{1}{-3}x^{-3}+c$
$\frac{1}{-12\cdot x^3}+c$
4. $\intcos(2x)dx=\frac{1}{2}\int(2\cdot cos(2x))dx=\frac{1}{2}sin(2x)+C$
5. $\int \frac{x^3-1}{x^2}dx=\int(\frac{x^3}{x^2}-\frac{1}{x^2})dx=\int(x-x^{-2})dx=\frac{1}{2}x^2-\frac{1}{-1}x^{-1}+c$
$=\frac{1}{2}x^2+\frac{1}{x}+c$
6. $\int e^{3x}dx=\frac{1}{3}\int(3\cdot e^{3x})dx$
$D(3x)=3 and 3 drops off as integration$
$\frac{1}{3}\cdot e^{3x}+c$
7. $\int\frac{3}{\sqrt{x}}=3\intx^{-1/2}dx=3\cdot(\frac{1}{1/2}x^{-1/2+1})$
$=3\cdot\frac{2}{1}x^{1/2}+c=6\sqrt{x}+c$

\end{document}
