\documentclass{article}
\usepackage{graphicx} % Required for inserting images
\usepackage{hyperref}
\usepackage{mathtools,amssymb,amsthm}

\title{The day's notes}
\author{Samuel Hautam√§ki}
%\date{October 2025}
\begin{document}
\subsection{Revision}
\obeylines
1. L'Hopital's 
$\lim_{x\to0}\frac{2sin x-sin 2x}{x^3}=\frac{2\cdot sin 0-sin 2\cdot0}{0^3}=\frac{0-0}{0}$
L'Hopital's rule 
$\lim_{x\to0}(\frac{2cos(x)-cos(2x\cdot 2}{2\cdot x})=subst..$
$=\frac{2\cdot1-1\cdot2}{2\cdot0}=\frac{0}{0}$
L'Hopital's rule
$\lim_{x\to0}(\frac{2(-sin(x))-2\cdot (-sin(2x))\cdot 2}{2})$
$=\frac{-2\cdot 1+4\cdot 0}{2}=-1$
$\lim_{x\to0}(\frac{2(-sin(x))-2\cdot(-sin(2x))\cdot 2}{3\cdot 2x})=\frac{0}{0}$
L'Hopital's rule
$\lim_{x\to0}(\frac{-2\cdot cos(x)+4\cdot cos(2x)\cdot2}{6})$
$\frac{-2\cdot 1+8\cdot1}{6}=\frac{6}{6}=1$ Ans: 1
2a. Use formula booklet for $cos(x)=1-\frac{x^2}{2!}+\frac{x^4}{4!}+...$
$ln(1+x)=x-\frac{x^2}{2}+\frac{x^3}{3}-...$
now $cos(ln(1+x))=1-\frac{(x-\frac{x^2}{2}+\frac{x^3}{3}-...)}{2!}+\frac{(x-\fracx^2}{2}+\frac{x^3}{3}-...)^4-$
binomial theorem
$=1-\frac{1}{2}\cdot(x^2-\frac{1}{2}x^3+\frac{1}{3}x^3-\frac{1}{4}x^4+...)$


\end{document}
