\documentclass{article}
\usepackage{graphicx} % Required for inserting images
\usepackage{hyperref}
\usepackage{graphicx} % Required for inserting images
\usepackage{mathtools,amssymb,amsthm}

\title{The day's notes}
\author{Samuel Hautam√§ki}
%\date{October 2025}
\begin{document}
\subsection{Constructing polynomials, Maclaurin and Taylor polynomial.}
HL p 554
\obeylines

Taylor series is expansion of $f(x)$ about point
$x=a$ 
$f(x)=f(a)+\frac{f'(a)}{1!}\cdot x^1+\frac{f''(a)}{2!}\cdot x^2+...+\frac{f^{(n)}(a)}{n!}\cdot x^n$
When point $x=0$ it's called Maclaurin series expansion of $f(x)$. (See formula booklet)
Lagrange form of error term $=remainder$
$R_n(x:a)=\frac{f^{(n+1)}(c)\cdot(x-a)^{n+1}}{(n+1)!}$
where $x\leq c\leq a$.
Example
Find 4th degree (=order) Maclaurin series of 
a) $sin(x)$
$f(0)=sin(0)=0$
$f'(x)=D sin(x)=cos(x)$ and $f'(0)=cos(0)=1$
$f''(x)=D cos(x)=-sin(x),f''(0)=-sin(0)=0$
$f'''(x)=D-sin(x)=-cos(x),f'''(0)=-cos(0)=-1$
$f^{(4)}(x)=D-cos(x)=-(-sin(x))=sin(x),f^{(4)}(0)=sin(0)=0$
so up to 4th degree there is $sin(x)\approx f(0)+\frac{f'(0)}{1!}x+\frac{f''(0)}{2!}x^2+\frac{f'''(0)}{3!}x^3+\frac{f^{(4)}(0)}{4!}x^4$
$=0+\frac{1}{1}x+\frac{0}{2}x^2+\frac{-1}{1\cdot 2\cdot 3}x^3+\frac{0}{6\cdot 4}x^4$
$=x-\frac{1}{6}x^3$
Graph the $sin(x)$ and the Maclaurin polynomial at $x=0$
p 556 ex 1,2
1. 
a) $f(x)=xe^x$
$f(0)=0\cdot e^0=0$
$f'(x)=1\cdot e^x+x\cdot e^x$ product rule
$f'(0)=1\cdot e^0+0\cdo te^0=1\cdot 1+0=1$
$f''(x)=D(e^x+x\cdot e^x)=e^x+1\cdot e^x+x\cdot e^x$
$f''(0)=e^0+e^0+0\cdot e^0=1+1=2$
$f'''(x)=D(2e^x+x\cdot e^x)=2\cdot e^x+(1\cdot e^x+x\cdot e^x)$
$f'''(0)=3\cdot e^0+0\cdot e^0=3\cdot 1+0=3$
$f^{(4)}(x)=D(3e^x+x\cdot e^x)=3e^x+1\cdot e^x+x\cdot e^x$
$f''''(0)=4\cdot1=4$
4th order Maclaurin polynomial is
$f(0)+\frac{f'(0)}{1!}x+\frac{f''(0)}{2!}x^2+\frac{f'''(0)}{3!}x^3+\frac{f^{(4)(0)}}{4!}x^4$
$=0+\frac{1}{1}x+\frac{2}{2}x^2+\frac{3}{6}x^3+\frac{4}{24}x^4$
$=x+x^2+\frac{1}{2}x^3+\frac{1}{6}x^4$.

Binomial series is Maclaurin expansion for $f(x)=(1+x)^p$
$=1+px+\frac{p(p-1)}{2!}x^2+\frac{p(p-1)(p-2)}{3!}x^3+...$
Example
Use the binomial series to find Maclaurin series of 
$a) f(x)=\frac{1}{(1+x)^2}$
$=(1+x)^{-2}$ where $p=-2$
$=1+px+\frac{p(p-1)}{2!}x^2+\frac{p(p-1)(p-2)}{3!}x^3+...$ subst.
$=1-2x-\frac{2(-2-1)}{2}x^2-\frac{2(-2-1)(-2-2)}{6}x^3+...$
$=1-2x+3x^2-4x^3+...$
Has form of $\sum_{n=0}^{\infty}((-1)^n\cdot (n+1)\cdot x^n)$.
p 562 ex 5a
5a) $f(x)=\sqrt{1-x}=(1-x)^{1/2}=(1+(-x))^{1/2}$
binomial series see formula booklet, $p=1/2$.
$=1+px+\frac{p(p-1)}{2!}x^2+\frac{p(p-1)(p-2)}{3!}x^3+...$subst
$=1+\frac{1}{2}(-2)+\frac{-1/2\cdot(-1/2-1)}{2}x^2+\frac{-1/2\cdot(-3/2)\cdot(-1/2-2)}{6}x^3+\frac{-1/2(-3/2)\cdot(-5/2)\cdot(-1/2-3)}{24}x^4+...$
$=1-\frac{1}{2}x+\frac{1}{8}x^2+\frac{1}{16}x^3+\frac{5}{128}x^4+...$



1a



\end{document}
