\subsection{Quadratic function}

$a\cdot x^2+b\cdot x+c=0$
Zeroes:
$x=\frac{-b\pm\sqrt{b^2-4\cdot a\cdot c}}{2\cdot a}$

$\Delta=discriminant$
$\Delta=b^2-4ac<0$ no roots in $\mathbb{R}$(realnumbers)
$\Delta=0$ there is one root.
$\Delta>0, 2 roots$

$(a+b)^2=a^2+2ab+b^2$
p 152 3B. 1.a)
$x^2+bx-7=0 ||+3^2$
$(x^2+2x\cdot 3+3^2)-7=3^2$
$(x+3)^2-7=9$
$(x+3)^2=16$ $||\pm\sqrt{}$
$x+3=4$ or $x=+3=-4$
$x=1$ or $x=-7$

HL p 159
1. a) $a=1, b=3, c=-7$
$(3)^2+(-4\cdot 1\cdot -7)=37$ has two roots 
b) $a=1 b=1 c=2$
$1^2+(-4\cdot 1\cdot 2)=-7$ no roots.
c) $a=1,b=2,c=1$
$2^2+(-4\cdot 1\cdot 2)=-4$ no roots
d) $a=5,b=\sqrt{3}+2$
$(\sqrt{3})^2+(-4\cdot 5\cdot 2)=-37$ no roots
e) $a=2, b=-\pi, c=1$
$(-\pi)^2+(-4\cdot 2\cdot 1)=1.8696$ has two roots.
f) $a=2.25, b=-21, c=49$
$(-21)^2+(-4\cdot 2.25\cdot 49)=0$ has 1 root.

\subsection{Viete's theorem}
Sum of roots of quadratic equation
$x_1+x_2=\frac{-b}{a}$ and $ax^2+bx+c=0, a\neq 0$

and product of roots.
$x_1\cdot x_2=\frac{c}{a}$

Direct proof (sum):
$x_1+x_2=\frac{-b+\sqrt{b^2-4ac}}{2a}+\frac{-b-\sqrt{b^2-4ac}}{2a}$
$\frac{-2b}{2a}=\frac{-b}{a}$

Direct proof (prod):
$x_1\cdot x_2=\frac{-b+\sqrt{b^2-4ac}}{2a}\cdot\frac{-b-\sqrt{b^2-4ac}}{2a}$
$=\frac{(-b+\sqrt{})\cdot (-b-\sqrt{})}{4a^2}$
$=\frac{(-b)^2-(\sqrt{b^2-4ac})^2}{4a^2}$
$=\frac{b^2-b^2+4ac}{4a^2}=\frac{4ac}{4a^2}=\frac{c}{a}$

hl p160 ex 1,2 and p 152 ex 1,2
3E. 1. 
$a=1, b=6, c=8$
$x=\frac{-6\pm\sqrt{(-6)^2-4\cdot 1\cdot 8}}{2}$
$x=\frac{-6\pm\sqrt{36-4\cdot 8}}{2}$ 
$x=\frac{-6\pm\sqrt{36-32}}{2}$
$x=\frac{-6\pm\sqrt{4}}{2}$
$x=\frac{-6+2}{2}=-2$
$x=\frac{-6-2}{2}=-4$

2. $polyRoots(x^2-8\cdo x+16,x)={4,4}$
P 152
1. b) $x^2-7x-30=0$
$x^2-7x=30$

