\documentclass{article}
\usepackage{graphicx} % Required for inserting images
\usepackage{hyperref}
\usepackage{graphicx} % Required for inserting images
\usepackage{mathtools,amssymb,amsthm}

\title{The day's notes}
\author{Samuel HautamÃ¤ki}
%\date{October 2025}
\begin{document}
\subsection{Paper 3}
Paper 3
\obeylines
2.
a) $L(x)=2x-1$ has $m=2,r=$root/solution of $2x-1$
$2x-1=0$
$2x=1$
$x=\frac{1}{2}$ $c=-1$
so arithmetic sequence $2,\frac{1}{2},-1,...$
common difference $d=u_2-u_1=$ or $u_3-u_2$.
$\frac{1}{2}-2=\frac{-3}{2}$ $-3-\frac{1}{2}=\frac{-3}{2}$
so $L(x)=2x-1$ is AS-linear.$\square$
b) i) $L(x)=m\cdot x+c$
r is root of $L(x)=0$ subst.
$m\cdot x+c=0$
$x=\frac{-c}{m}$, so root $r=\frac{-c}{m}$.$\square$
ii) so $L(x)=m\cdot x+c=$ and $r=-\frac{c}{m}$
-> $m\cdot r=c$ and $c=-mr$
so $L(x)=m\$
t x+c=m\cdot x-m\cdot r$
and the root $r=?$
$m\cdot x-m\cdot r=0$
$mx=mr$ 
$x=r$
so $L(x)=0$ at $x=r$
NOW $L(x)=m\cdot x-\frac{m^2}{m+2}$ so $r=\frac{-c}{m}=subst=\frac{--\frac{m^2}{m+2}}{m}=\frac{-m^2}{m+2}\cdot(\frac{1}{m})=\frac{m}{m+2}$
so subst. $x=\frac{m}{m+2}$ gives $L(x)=0$
$L(\frac{-m}{m+2})=(m\cdot (\frac{m}{m+2})-\frac{m^2}{m+2})=0$ that is AS-linear.$\square$
iii) $m+2\neq0,m\neq-2$
c) $L(x)=-x-1$has arithmetic sequence.
$m=-1$, $r=\frac{-c}{m}=subst.\frac{-(-1)}{-1}=-1$ and $c=-1$
$-1,-1,-1,-1,-1$
and 2nd AS-linear $L(x)=mx-\frac{m^2}{m+2}=subst$
$=-1x-\frac{(-1)^2}{-1+2}=-x-1$ the same
so trial and error
sequence $m,\frac{-c}{m},c$
$m      \frac{-c}{m}$        $c$
yes/no arithmetic.
only integer.
$1 -1 1$ no
$-3 3 9$ yes d=6
$4 -2 8$ no
$-4 2 8$ yes $d=6$
Ans: $m=-3,r=3$ and $c=9$ or $m=-4,r=2,c=8$

d) $Q=(x)=a\cdot x^2+b\cdot x+c=0$ has root $r_1$, $r_2$
i) sum of roots $r_1+r_2=\frac{-b+\sqrt{b^2-4ac}}{2a}+\frac{-b-\sqrt{b^2-4ac}}{2a}=\frac{-b}{a}$
ii) product of roots
$r_1\cdot r_2=\frac{-b+\sqrt{b^2-4ac}}{2a}\cdot\frac{-b-\sqrt{b^2-4ac}}{2a}$
$=\frac{(-b)^2-(\sqrt{b^2-4ac})^2}{-4a^2}=\frac{b^2-(b^2-4ac)}{4a^2}=\frac{c}{a}$
e) $a,r_1,b,r_2,c$ are in arithmetic sequence
that means cd $d=r1-a=b-r1=r2-b=c-r2$
$r1-a=b-r1=2r_1=b+a$
$r_1=\frac{a+b}{2}$ and $b-r1=r2-b$
$2\cdot b-\frac{a+b}{2}=r_2$
NOW $r_2-r_1=subst=(2\cdot b-\frac{a+b}{2})-\frac{a+b}{2}$
$=2b-2\cdot(\frac{a+b}{2})=2b-(a+b)=b-a\square$
ii) note the memory formula $(A+B)(A-B)=A^2-B^2$
so $(r_2+r_1)\cdot(r_2-r_1)$ subst di and ei
$=(\frac{-b}{a})\cdot(b-a)=\frac{-b^2+2ab}{a}$ not this but
$\begin{cases}r_2-r_1=b-a\\r_2+r_1=\frac{-b}{a}\end{cases}$
$-2r_1=(b-a)-(\frac{-b}{a})$
$-2r_1=\frac{ba-a^2+b}{a}$
$r_1=\frac{a^2-ba-b}{2a}\square$



\end{document}
