\subsection{Powers and roots of complex numbers}
"easy case" p 172

Example. Find $z^3$ where $z=(2+3i)$
$z\cdot z^2=$ or $(2+3i)^3$ binomial formula.
$=nCr(3,0)2^3\cdot(3i)^0+nCr(3,1)2^2(3i)^1+nCr(3,2)2^1(3i)^2+nCr(3,3)2^0(3i)^3$
$=1\cdot 8\cdot 1+3\cdot 4\cdot 3i+3\cdot 2\cdot 9\cdot i^2+1\cdot 1\cdot 27\cdot i\cdot i^2$
$=8+36i-54-27i$ since $i^2=-1$
$=-46+9i$
(or calculator in paper 2)

Example b) Find or evaluate = do the calculations $\sqrt{2+3i}$.
Lets mark $z=\sqrt{2+3i} || ()^2$
$z^2=2+3i$
$(a+bi)^2=2+3i$
$a^2+2abi+b^2i^2=2+3i$
$a^2-b^2=2$ (real part)
$2abi=3i$ (imaginary part)
$\begin{cases}
a^2-b^2=2 \\ 2ab=3 \end{cases}$
substitute from row below.
$b=\frac{3}{2a}$ subst.
$a^2-(\frac{3}{2a})^2=2$
$\frac{a^2}{1}-\frac{9}{4a^2}=2$
$\frac{4a^4-9}{4a^2}=2$
$4a^4-9=8a^2$
$t=a^2,a^4=t^2$
$4t^2-8t-9=0$
$x=\frac{-(-8)\pm\sqrt{\sqrt{-8}^2-4\cdot 4(-9}}{2\cdot 4}$
$\frac{8\pm\sqrt{64+72}}{8}$
$=\frac{8\pm2\sqrt{34}}{8}=\frac{2(4\pm(34)}{2\cdot 4}=\frac{4\pm\sqrt{34}}{4}$
subst. back
$t=a^2$
$a^2=\frac{4\pm\sqrt{34}}{4} ||\pm$
$a=\pm\sqrt{\frac{4\pm\sqrt{34}}{4}}=\pm\frac{\sqrt{4\pm\sqrt{34}}}{2}$
$and b=\frac{3}{2a}=\frac{3}{2(\pm(\frac{\sqrt{4\pm\sqrt{34}}}{2}))}$
Ans; $z=\sqrt{2+3i}=\frac{\sqrt{4\pm\sqrt{34}}}{2}+i\cdot\frac{3}{\sqrt{4\pm\sqrt{34}}}$
$z_2=\frac{-\sqrt{4\pm\sqrt{34}}}{2}-i\cdot\frac{3}{\sqrt{4\pm\sqrt{34}}}$
Note
$z=\sqrt[n]{(a+bi)} || ()^n$
$(re+i\cdot Im)^n=a+bi$
binomial formula and pair of equations
$\begin{cases}real part left = RHS \\ imaginary part LHS = RHS\end{cases}$
Ans: n different solutions.

A calculator can be used to evaluate square root, but the calculator will noly give one solution. Have to remember that the second solution is the opposite number.

P 174 3H
1. a) $i^7 + i^17 + i^27 + i^37$
$i^2\cdot i^2i^2\cdot i^1+(i^4)\cdot i^4\cdot i^4\cdot i^3+(i^4)^9\cdot i^1$
$=(-1)\cdot(-1)\cdot(-1)\cdot 1+1\cdot 1\cdot 1\cdot 1 \cdot i \cdot i^2+1^6i^1i^3+1^6\cdot i$
$=-i +i -1i + i =0$
Calculator =0
b)
c) $(3+i^77)\cdot (1-2i^{93})=3\cdot 1+3\cdot (-2i)^{93}+(i^77)\cdot 1+(i^77)\cdot (-2i)^{93}$
d)
e) $\frac{\sum_{k=1}^{2019}i^k}{\prod_{k=1}^{2019}i^k}=\frac{i+i^2+i^3+i^4+...+i^2019}{i\cdot i^2\cdot i^3\cdot i^4...i^{2019}}$
$=\frac{geometric sum}{i^{1+2+3+...+2019}}=\frac{geometric sum}{i^{arithmetic sum}}$
$=\frac{\frac{i\cdot(1-i^{2019})}{1-i}}{i^{(\frac{1+2019}{2}\cdot2019)}}$
$=\frac{\frac{1-1^{2020}}{1-i}}{i^{1005\cdot 2019}}$
$=\frac{\frac{i-1}{(-(i-1)}}{i^{2039190}}=\frac{-1}{i^2\cdot i^{4\cdot 509797}}=\frac{-1}{-1\cdot 1}=1$
Or calculator paper 2 $\frac{\sum_{k=1}^{2019}i^k}{\prod_{k=1}^{2019}i^k}=1$
