\documentclass{article}
\title{\LaTeX Math notes}
\author{Samuel Hautam√§ki}
\date{th of October 2024}
\usepackage{mathtools,amssymb,amsthm,gensymb,textcomp}
\begin{document}
  \maketitle
   
  \section{Derivative of inverse trigonometric functions + tangents and normals.}
  p 427\\
  Derivative of a function is the gradient (=slope) of tangent.\\ 
  $slope of tangent\cdot slope o fnormal=-1$\\
  tangent line $y-y_0=m\cdot(x-x_0)$\\
  where m=slope=$f'(x_0)$\\
  $y_0=f(x_0)$\\

  HL only: see formula booklet:\\
  $D arcsin (x)=\frac{1}{\sqrt{1-x^2}}$\\
  $D arccos (x)=\frac{-1}{\sqrt{1-x^2}}$\\
  $D arctan (x)=\frac{1}{1+x^2}$\\
  Example: $f(x)=arccos(2x)$\\
  $f'(x)=\frac{-1}{\sqrt{1-(2x)^2}}\cdot D(2x)$ chain rule.\\
  $=\frac{-2}{\sqrt{1-4x^2}}$\\
  b) $D arctan (2x+1)$\\
  $\frac{1}{1+(2x+1)^2}\cdot D (2x+1)=\frac{2}{1+4x^2+4x+1}=\frac{1}{2x^2+2x+1}$\\
  hl p 428: 1,2,3 only a,b\\
  +p431 ex 1\\
  1. a) $f(x)=arccos(2x)$\\
  $f'(x)=\frac{-1}{1-(2x)^2}\cdot D(2x)$\\
  $\frac{-2}{1-4x^2}$\\
  b) $f(x)=arcsin \frac{3}{2}x$\\
  $f'(x)=\frac{1}{1-(\frac{3}{2}x)^2}\cdot D(\frac{3}{2}x)$\\
  $\frac{3}{2}\cdot\frac{1}{1-(\frac{3}{2}x)^2}$\\
  2. a) $y=2x arccos x$\\
  $y'=2\cdot arccos x+\frac{-1}{\sqrt{1-x^2}}\cdot2x$\\
  b) $y=\frac{arccos x}{2x}=\frac{2x\cdot \frac{-1}{\sqrt{1-x^2}-arccos x\cdot 2}}{2x^2}$\\
  

   
\end{document}
