\documentclass{article}
\title{\LaTeX Math notes}
\author{Samuel HautamÃ¤ki}
\date{th of October 2024}
\usepackage{mathtools,amssymb,amsthm,gensymb,textcomp}
\begin{document}
  \maketitle
   
  \section{Equations of log and exponents}
  HL p 472\\
  paper 2 methods: graphs intersect x=$nsolve(equation,x,a guess)$\\
  paper 1 method:\\
  definition: $a^b=c   ===== log_a(c)=b$\\
  and rules of log and exponents\\
  Example. Solve a) $2\cdot5^x=200$\\
  $5^x=100$\\
  $log_5(100)=x=2.86$\\
  b) $x^{x-3}=16^x$\\
  equal base, equal exponents\\
  $2^{x-3}=(2^4)^x$\\
  $2^{x-3}=2^{4x} || log_2()$\\
  $x-3=4x$\\
  $x=-1$\\
  c) solve $e^x=17$\\
  $ln(e^x)=ln(17)$\\
  $x=ln(17)=2.83$\\
  d solve the inequality\\
  $6^x>3^{x+1} || ln() increasing function$\\
  $ln(6^x)>ln(3^x+1)$\\
  $x\cdot ln(6)>(x+1)\cdot ln(3)$\\
  $x ln 6 > x ln 30 ln3$\\
  $x ln 6 - x ln 3 > ln 3$\\
  $x\cdot(ln 6 - ln 3) > ln3$\\
  $x\cdot ln(\frac{6}{3})>ln 3$\\
  $x\cdot ln(2)>ln 3$\\
  $x>\frac{ln 3}{ln 2}$\\
  $x>log_2(3)$\\
  e) $3\cdot 2^x=4^x-10$ a tpical exam question!\\
  $3\cdot 2^x-(2^2)^x+10=0$\\
  $3\cdot2^x-2^{x\cdot2}+10=0$\\
  $-(2^x)^2+3\cdot(2^x)+10=0$\\ 
  lets substitute $t=2^x$\\
  $-t^2+3\cdot t+10=0$ qiadratic formula $a=-1,b3=,c=10$\\
  $t=\frac{-3\pm\sqrt{3-4\cdot(-1)\cdot10}}{2\cdot(-1)}=\frac{-3\pm\sqrt{9+40}}{-2}$\\
  $t=\frac{-3+7}{-2}=-2 or t=\frac{-3-7}{-2}=5$\\
  $t=2^x 2^x=-2$\\
  or $2^x=5$\\
  $x=log_2(-2)$\\
  no solution $log has domain >0$\\
  $x=log_2(5)$\\
  $=2.32$\\
  g) solve $log_4(x)=2$\\
  $x=16$\\
  h) $log_x(3)=\frac{1}{2}$\\
  $x^{\frac{1}{2}}=3$\\
  $x=3^2$\\
  $x=9$\\
  \subsection{copy 9L}
  HL page 472: 11-17,
  COPY 9L:
  1a) $2^x=5$\\
  $log_2(5)=x=2.32$\\
  b) $3^x=17$\\
  $log_3(17)=x=2.57$\\
  c) $9^x=49$\\
  $log_9(49)=x=1.77$\\
  d) $3^x=69$\\
  $log_3(69)=x=3.85$\\
  2a) $2^{4x}=9$\\
  $4x=log_2(9)$\\
  $x=\frac{log_29}{4}$\\
  2b) $6^{3x}=4$\\
  $3x=log_6(4)$\\
  $x=\frac{log_64}{3}=0.257$\\
  3a) $6\cdot 2^x=14$\\
  $2^x=\frac{14}{6}$\\
  $2^x=\frac{7}{3}$\\
  $x=log_2(\frac{7}{3})$\\
  $=1.222$\\
  3b) $3\cdot 6^{3x}=16$\\
  $6^{3x}=4$\\
  $3x=log_6(4)$\\
  $x=\frac{log_64}{3}$\\
  =$0.257$\\

  
  

\end{document}
