\documentclass{article}
\title{\LaTeX Math notes}
\author{Samuel Hautam√§ki}
\date{th of October 2024}
\usepackage{mathtools,amssymb,amsthm,gensymb,textcomp}
\begin{document}
  \maketitle
   
  \section{Derivativse of logarithms and exponentials}
  HL p 477\\
  $D e^x=e^x$\\
  $D a^x=a^x\cdot ln(a)$\\
  $D e^{f(x)}=chain rule =e^{f(x)}\cdot f'(x)$\\
  $D ln(x)=\frac{1}{x}$\\
  $D log_a(x)=\frac{1}{x\cdot ln(a)}$\\
  $D ln(f(x))=\frac{1}{f(x)}\cdot f'(x)$ chain rule\\
  Example a) differentiate $f(x)=e^{x^2-3x}$\\
  that is fid the derivative\\
  $f'(x) D e^{x^2-3x}=e^(x^2-3x)\cdot(2x-3)$\\
  b) $g(x)=\frac{2}{\sqrt[3]{e^x}}$\\
  $g'(x)=D (2\cdot e^{-x/3})=2\cdot e^{-x/3}\cdot (D(-x/3))$\\
  $=2\cdot e^{-x/3}\cdot(-\frac{1}{3})=\frac{-2}{3\cdot\sqrt[3]{e^x}}$\\
  c) $h(x)=\frac{3^{2x}-e^x}{x^2}$\\
  $h'(x)=\frac{(e^{(2x)}\cdot x^2-(2^{2x}-e^x)\cdot 2x)}{(x^2)^2}$\\
  $=\frac{2xe^{2x}-xe^x-2e^2x+2e^x}{x^3}$\\
  d) $D ()3^x+x^3-\frac{1}{x^3}$\\
  $3^x\cdot ln(3)+3x^2- Dx^-3$\\
  $3^x\cdot ln(3)+3x^2-(-3)x^4$\\
  $3^x\cdot ln(3)+3x^2+\frac{3}{x^4}$\\
  hl p 487 ex: 1-4 + copy sl p 424\\
  1. a) $y=3e^{5x+4}$\\
  $3e^{5x+4}\cdot (5)$\\
  b) $y=e^{3x^2}$\\
  $y'=e^{3x^2}\cdot 6x$\\
  c) $y=5^{4x}$\\
  $y'=5^{4x}\cdot 4$\\
  d) $y=e^{cos(x)}$\\
  $y'=e^{cos(x)}\cdot (-sin(x))$\\
  e) $e=ln(\sqrt{x})$\\
  $D ln(x^{1/2})=\frac{1}{x^{1/2}}\cdot D(x^{1/2})$\\
  $=\frac{1}{x^{1/2}}\cdot (\frac{1}{2}x^{-1/2})$\\
  $\frac{1}{2\sqrt{x}\cdot\sqrt{x}}=\frac{1}{2\cdot x}$\\
  f) $y=3-5 ln(x)$\\
  $y'=-5\cdot ln(x)$\\
  $5\cdot\frac{1}{x}$\\
  g) $y=ln(5x+4)$\\
   


\end{document}
