\documentclass{article}
\title{\LaTeX Math notes}
\author{Samuel Hautamäki}
\date{th of October 2024}
\usepackage{mathtools,amssymb,amsthm,gensymb,textcomp}
\begin{document}
  \maketitle
   
  \section{equations with exponents}
  HL p 464 \\
  Solve the equations\\
  a) $x^3=-27 || \sqrt[3]{}$ for odd only one answer\\
  $x=\sqrt[3]{-27}$\\
  $x-3$\\
  b) $x^2-16=0$\\
  $x^2=16$ for even roots $\pm$\\
  $x=\pm4\\$
  c) $3^{2x+1}=9$\\
  $3^{2x+1}=3^2$ same base equal exponents\\
  $2x+1=2$\\
  $2x=1$\\
  $x=\frac{1}{2}$\\
  d) $2^x=15 || log_2()$\\
  $log_2(2^x)=log_2(15$\\
  $x=log_2(15)=3.90689$\\
  or $nsolve()$\\
  NOTE $a^x=b \leftrightarrow x = \log_a(b)$\\
  HL ex 464 ex6+ p514 ex 1\\ 
  1. a) $(81)^\frac{3}{4}$\\
  $\sqrt[4]{81^3}$\\
  $=1062882$\\
  b) $(\frac{8}{125})^{\frac{1}{3}}$\\
  $\sqrt[3]{\frac{8}{125}^1}$\\
  c) $(\frac{32}{243})^{\frac{2}{5}}$\\
  $\sqrt[5]{(\frac{32}{243}^2)}$\\
  $=0$\\
  2. a) $(\frac{a^{12}y^{-3}}{16y})^{\frac{3}{4}}=\frac{a^9}{8y}$\\
  6.
  a) $2^{3x}-2^{7x-2}=0$\\
  $2^{x+2}-2^{1-x}=7$\\
  $2^2\cdot 2^x-\frac{2}{2x}=7$\\
  $4\cdot(2^x)^2-2=7\cdot 2^x$\\
  $4\cdot t^2+7t-2=0$\\
  $\frac{-(7)\pm\sqrt{7^2-4\cdot4\cdot-2}}{2\cdot4}$\\
  $\frac{(-7)\pm\sqrt{49+32}}{8}$\\
  $\frac{(-7)\pm\sqrt{81}}{8}$\\
  $\frac{(-7)\pm9}{8}$\\
  $t=$
  c) $9^x+9=10\cdot 3^x$\\
  $3^{2\cdot x}+010\cdot 3^x=0$\\
  $(3^x)^2-10\cdot(3^x)+9=0$ quadratic formula let's $t=3^x$ gives $t^210\cdot t+9=0$\\
  $1,b=-10,c=9$\\
  $t=\frac{-(-10)\pm\sqrt{-10^2-4\cdot 1\cdot 9}}{2}$\\
  $\frac{10\pm\sqrt{64}}{2}$\\
  $\frac{10\pm8}{2}$\\
  $\frac{10-8}{2}=1, \frac{10+8}{2}=9$\\
  $3^x=9$\\
  $3=3^2$\\
  $3^x=1$\\
  $3^x=3^0$\\
  $x=2$ or $x=0$\\
   

   
\end{document}
