\documentclass{article}
\title{\LaTeX Math notes}
\author{Samuel Hautam√§ki}
\date{2nd of September 2024}
\usepackage{mathtools,amssymb,amsthm,gensymb,textcomp}
\begin{document}
  \maketitle
   
  \section{Chain rule}
  Chain rule of differentiation\\
  HL p 254\\
  $D F ( G(x)) = F'(G(x)) \cdot G'(X)$\\
  formula booklet: $\frac{dy}{dx}=\frac{dy}{du}\cdot\frac{du}{dx}$\\
  so derivate outer function and just mark the inner function and later do product with inner function's derivative only.\\
  
  Example a) $D(2x^3+4x)^7=7\cdot(2x^3+5x)^6\cdot D(2x^3+5x)$\\
  $=7\cdot(2x^3+5x)^6\cdot(6x^2+5)$\\
  b) $h(x)=\sqrt{2x-3}$\\
  $h'(x)=?=D (2x-3)^(\frac{1}{2})=\frac{1}{2}\cdot(2x-3)^(-\frac{1}{2})\cdot2$\\
  $=\frac{1}{\sqrt{2x-3}}$\\
  \section{p254ex1-6}
  1. a. $y=(4x-3)^5$\\
  $5\cdot(4x-3)^4\cdot(4)$\\
  b. $y=\sqrt{1-4x}$
  $\frac{1}{2}\cdot(1-4x)^(-\frac{1}{2})\cdot4$\\
  c. $y=\frac{2-x^2-3x^5}{x}$\\
  $\frac{dy}{dx}=D(\frac{2-x^2-3x^5}{x})=D(\frac{2}{x}-\frac{2x^2}{x}-\frac{3x^5}{x})$\\
  $=D(2\cdot x{^-1}-x-3x^4$\\
  $=2\cdot(-1)x^{-2}-1-3\cdot4x^3$\\
  $=\frac{-2}{x^2}-1-12x^3$\\
  d.  

   
\end{document}
