\documentclass{article}
\title{\LaTeX Math notes}
\author{Samuel Hautam√§ki}
\date{26th of August 2024}
\usepackage{mathtools,amssymb,amsthm,gensymb,textcomp}
\begin{document}
  \maketitle
   
  \section{Differentiation rules}
  HL p 249.\\
  1) Constant function $f(x)=constant c$ has $f'(x)=0$\\
  since slope of tangent is 0.
  2) line $f(x)=a\cdot x+c$\\
  $f'(x)=a+0=a$\\
  3) power function $f(x)=x^n$\\
  $f'(x)=n\cdot x^{n-1}$\\
  4) sum and difference of $f(x)=u(x)\pm v(x)$\\
  $f'(x)=u'(x)\pm v'(x)$\\
  differentiate term by term only if + or -.\\
  Note product and division has their own rules, so try to simplify into polynomials.\\
  Example differentiate the following:\\
  a) $f(x)=5^2+4x+7$\\
  $f'(x)=5x^4+4$\\
  b) $f(x)=\sqrt{x}\cdot x = x^\frac{1}{2}\cdot x^1=x^{1+\frac{1}{2}}=x^\frac{3}{2}$\\
  $f'(x)=D x^{\frac{3}{2}}=\frac{3}{2}\cdot x^{\frac{1}{2}}=\frac{3}{2}\cdot\sqrt{x}$\\
  c) $f(x)=\frac{x^2-4}{x+2}=\frac{(x-2)(x+2)}{x+2}=x-2$\\
  $f'(x) = D (x-2)=1$\\
  Ex. 252 p 1-7\\
  1. a. $(3x-1)^2$\\
  $f'(x)=(3x)^2-2\cdot 3x\cdot 1+1^2$\\
  $=\frac{d}{dx}(9x^2-6x+1)=9\cdot 2x^1=18$\\
  b. $3x^5-4x^2+2x-1$\\
  $\frac{d}{dx}(5\cdot 3x^4-2\cdot 4x)$\\
  $15x^4-8x=2$\\
  c.  
  

   
\end{document}
